src/SDK/Serialize/SerializableTypes.dfy
@@ -4,14 +4,12 @@
 include "../../Util/UTF8.dfy"
 include "../../Generated/AwsCryptographicMaterialProviders.dfy"
 include "../../StandardLibrary/StandardLibrary.dfy"
-include "../../AwsCryptographicMaterialProviders/Client.dfy"
 
 module SerializableTypes {
   import StandardLibrary
   import opened UInt = StandardLibrary.UInt
   import opened UTF8
   import opened Aws.Crypto
-  import MaterialProviders.Client
 
   type ShortUTF8Seq = s: ValidUTF8Bytes | HasUint16Len(s)
 
@@ -86,21 +84,6 @@ module SerializableTypes {
   lemma LemmaSupportedAlgorithmSuitesIsComplete(id:Crypto.AlgorithmSuiteId)
     ensures id in SupportedAlgorithmSuites
   {}
-
-  lemma LemmaESDKAlgorithmSuiteIdImpliesEquality(
-    esdkId: ESDKAlgorithmSuiteId,
-    suite: Client.AlgorithmSuites.AlgorithmSuite
-  )
-    requires GetAlgorithmSuiteId(esdkId) == suite.id
-    ensures
-      && var suiteId := GetAlgorithmSuiteId(esdkId);
-      && Client.SpecificationClient().GetSuite(suiteId) == suite
-  {
-    var suiteId := GetAlgorithmSuiteId(esdkId);
-    if Client.SpecificationClient().GetSuite(suiteId) != suite {
-      assert Client.SpecificationClient().GetSuite(suiteId).encrypt.keyLength == suite.encrypt.keyLength;
-    }
-  }
 
   /*
    * Length properties
